module Naturals where

data â„• : Set where
  zero : â„•
  suc  : â„• â†’ â„•
{-# BUILTIN NATURAL â„• #-}

seven : â„•
seven = suc (suc (suc (suc (suc (suc (suc zero))))))

import Relation.Binary.PropositionalEquality as Eq

open Eq using (_â‰¡_; refl)
open Eq.â‰¡-Reasoning using (begin_; _â‰¡âŸ¨âŸ©_; _âˆ)

_+_ : â„• â†’ â„• â†’ â„•
zero    + n = n
(suc m) + n = suc (m + n)

_ : 2 + 3 â‰¡ 5
_ =
  begin
    2 + 3
  â‰¡âŸ¨âŸ© -- is shorthand for
    (suc (suc zero)) + (suc (suc (suc (zero))))
  â‰¡âŸ¨âŸ© -- inductive case
    suc ((suc zero) + (suc (suc (suc zero))))
  â‰¡âŸ¨âŸ© -- inductive case
    suc (suc (zero + (suc (suc (suc zero)))))
  â‰¡âŸ¨âŸ© -- base case
    suc (suc (suc (suc (suc zero))))
  â‰¡âŸ¨âŸ© -- is longhand for
    5
  âˆ

_ : 2 + 3 â‰¡ 5
_ = refl

_*_ : â„• â†’ â„• â†’ â„•
zero    * n = zero
(suc m) * n = n + (m * n)

_^_ : â„• â†’ â„• â†’ â„•
m ^ zero    = suc zero
m ^ (suc n) = m * (m ^ n)

_ : 3 ^ 4 â‰¡ 81
_ =
  begin
    3 ^ 4
  â‰¡âŸ¨âŸ© -- applying ^
    3 * (3 ^ 3)
  â‰¡âŸ¨âŸ© -- applying ^
    3 * (3 * (3 ^ 2))
  â‰¡âŸ¨âŸ© -- applying ^
    3 * (3 * (3 * (3 ^ 1)))
  â‰¡âŸ¨âŸ© -- applying ^
    3 * (3 * (3 * (3 * (3 ^ 0))))
  â‰¡âŸ¨âŸ© -- base case
    3 * (3 * (3 * (3 * 1)))
  â‰¡âŸ¨âŸ© -- applying *
    3 * (3 * (3 * 3))
  â‰¡âŸ¨âŸ© -- applying *
    3 * (3 * 9)
  â‰¡âŸ¨âŸ© -- applying *
    3 * 27
  â‰¡âŸ¨âŸ© -- applying *
    81
  âˆ

_-_ : â„• â†’ â„• â†’ â„•
m     - zero  = m
zero  - suc n = zero
suc m - suc n = m - n

infixl 6 _+_ _-_
infixl 7 _*_

{-# BUILTIN NATPLUS _+_ #-}
{-# BUILTIN NATTIMES _*_ #-}
{-# BUILTIN NATMINUS _-_ #-}

-- Binary Representation of number
data Bin : Set where
  âŸ¨âŸ© : Bin
  _ğŸ˜ : Bin â†’ Bin
  _ğŸ™ : Bin â†’ Bin

eleven : Bin
eleven = âŸ¨âŸ© ğŸ™ ğŸ˜ ğŸ™ ğŸ™

ceil : Bin -> Bin
ceil âŸ¨âŸ© = âŸ¨âŸ© ğŸ™
ceil (m ğŸ˜) = (ceil m) ğŸ˜
ceil (m ğŸ™) = (ceil m) ğŸ˜

inc : Bin â†’ Bin
inc âŸ¨âŸ© = âŸ¨âŸ© ğŸ™
inc (âŸ¨âŸ© ğŸ˜) = âŸ¨âŸ© ğŸ™
inc (âŸ¨âŸ© ğŸ™) = âŸ¨âŸ© ğŸ™ ğŸ˜
inc ((m ğŸ˜) ğŸ˜) = (m ğŸ˜) ğŸ™
inc ((m ğŸ˜) ğŸ™) = (m ğŸ™) ğŸ˜
inc ((m ğŸ™) ğŸ˜) = (m ğŸ™) ğŸ™
inc ((m ğŸ™) ğŸ™) = ceil ((m ğŸ™) ğŸ™)

to : â„• â†’ Bin
to zero    = âŸ¨âŸ© ğŸ˜
to (suc n) = inc (to n)

from : Bin â†’ â„•
from âŸ¨âŸ© = zero
from (m ğŸ˜) = 2 * from m
from (m ğŸ™) = 2 * from m + 1

_ : from eleven â‰¡ 11
_ =
  begin
    from eleven
  â‰¡âŸ¨âŸ© -- applying from
    2 * from (âŸ¨âŸ© ğŸ™ ğŸ˜ ğŸ™) + 1
  â‰¡âŸ¨âŸ© -- applying from
    2 * (2 * from (âŸ¨âŸ© ğŸ™ ğŸ˜) + 1) + 1
  â‰¡âŸ¨âŸ© -- applying from
    2 * (2 * (2 * from (âŸ¨âŸ© ğŸ™)) + 1) + 1
  â‰¡âŸ¨âŸ© -- applying from
    2 * (2 * (2 * (2 * from âŸ¨âŸ© + 1)) + 1) + 1
  â‰¡âŸ¨âŸ© -- base case
    2 * (2 * (2 * (2 * 0 + 1)) + 1) + 1
  â‰¡âŸ¨âŸ© -- refl
    11
  âˆ

_ : inc (âŸ¨âŸ© ğŸ˜) â‰¡ âŸ¨âŸ© ğŸ™
_ = refl

_ : inc (âŸ¨âŸ© ğŸ™) â‰¡ âŸ¨âŸ© ğŸ™ ğŸ˜
_ = refl

_ : inc (âŸ¨âŸ© ğŸ™ ğŸ˜) â‰¡ âŸ¨âŸ© ğŸ™ ğŸ™
_ = refl

_ : inc (âŸ¨âŸ© ğŸ™ ğŸ™) â‰¡ âŸ¨âŸ© ğŸ™ ğŸ˜ ğŸ˜
_ = refl
